src/kemedhoc/Spec.KEMEDHOC.TranscriptHash.fst
@@ -1,6 +1,7 @@
 module Spec.KEMEDHOC.TranscriptHash
 
 module EdhocCrypto = Spec.EDHOC.CryptoPrimitives
+module Seq = Lib.Sequence
 
 open Spec.EDHOC.Serialization
 
@@ -11,10 +12,19 @@ let compute_th1 #kcs pk_X ct_auth_R
 /// Transcript Hash 2
 let compute_th2 #kcs ct_y k_auth_I msg1
   = let msg1_hash = do_hash kcs (concat_msg1 msg1) in
-  do_hash kcs (ct_y @< k_auth_I @< msg1_hash)
+  let input_hash = (ct_y @< k_auth_I @< msg1_hash) in
+  // let input_hash = Seq.concat (Seq.concat ct_y k_auth_I) msg1_hash in
+  (**) assert(
+    let concat_input_hash = Seq.concat (Seq.concat ct_y k_auth_I) msg1_hash in
+    Seq.equal input_hash concat_input_hash
+  );
+  do_hash kcs input_hash
 
 let compute_th2_pre_hash #kcs ct_y k_auth_I msg1_hash
-  = do_hash kcs (ct_y @< k_auth_I @< msg1_hash)
+  =
+  // let input_hash = Seq.concat (Seq.concat ct_y k_auth_I) msg1_hash in
+  let input_hash = (ct_y @< k_auth_I @< msg1_hash) in
+  do_hash kcs input_hash
 
 let lemma_compute_th2_equal_pre_hash #kcs ct_y k_auth_I msg1
   = ()
