src/kemedhoc/Impl.KEMEDHOC.TranscriptHash.fst
@@ -1,0 +1,141 @@
+module Impl.KEMEDHOC.TranscriptHash
+
+(*LowStar related modules*)
+module B = LowStar.Buffer
+module ST = FStar.HyperStack.ST
+module HS = FStar.HyperStack
+module S = FStar.Seq
+module Seq = Lib.Sequence
+
+(*Specification modules*)
+// module Spec = Spec.KEMEDHOC.TranscriptHash
+friend Spec.KEMEDHOC.TranscriptHash
+
+module SpecCrypto = Spec.KEMEDHOC.CryptoPrimitives
+module SpecParser = Spec.KEMEDHOC.Parser
+
+open Spec.EDHOC.Serialization
+
+/// Transcript Hash 1
+let compute_th1 #kcs pk_X ct_auth_R th1
+  = ST.push_frame ();
+  let input_len = (kem_public_key_size_t kcs +! kem_ciphertext_size_t kcs) in
+  let input_hash = create input_len (u8 0) in
+  concat_buff2 pk_X ct_auth_R input_hash;
+
+  do_hash kcs th1 input_len input_hash; 
+  ST.pop_frame();
+  ()
+
+/// Transcript Hash 2
+// #push-options "--z3rlimit 10"
+let compute_th2 #kcs ct_y k_auth_I msg1 th2
+  = (**) let h0 = ST.get () in
+  ST.push_frame ();
+  let msg1_len = concat_msg1_fixed_length_t kcs in
+  let msg1_buffer = create msg1_len (u8 0) in
+  concat_msg1 kcs msg1 msg1_buffer;
+  (**) let h1 = ST.get () in
+  (**) assert(modifies1 msg1_buffer h0 h1);
+
+  let msg1_hash_len = (size (SpecCrypto.hash_size kcs)) in
+  let msg1_hash = create msg1_hash_len (u8 0) in
+  do_hash kcs msg1_hash msg1_len msg1_buffer;
+  (**) let h2 = ST.get () in
+  (**) assert(modifies1 msg1_hash h1 h2);
+
+  let input_len = kem_ciphertext_size_t kcs +! kem_shared_secret_size_t kcs +! msg1_hash_len in
+  let input_hash = create input_len (u8 0) in
+  concat_buff3 ct_y k_auth_I msg1_hash input_hash;
+  (**) let h3 = ST.get () in
+  (**) assert(modifies1 input_hash h2 h3);
+
+  do_hash kcs th2 input_len input_hash;
+  (**) let h4 = ST.get () in
+  (**) assert(modifies1 th2 h3 h4);
+  (**) assert(
+    let msg1_s = message1_eval h0 msg1 in
+    let msg1_concat_s = SpecParser.concat_msg1 msg1_s in
+    let msg1_hash_s = SpecCrypto.do_hash kcs msg1_concat_s in
+    // let input_hash_s = Seq.concat (Seq.concat (as_seq h0 ct_y) (as_seq h0 k_auth_I)) msg1_hash_s in
+    let input_hash_s = (as_seq h0 ct_y) @< (as_seq h0 k_auth_I) @< msg1_hash_s in
+    let th2_s = SpecCrypto.do_hash kcs input_hash_s in
+
+    Seq.equal (as_seq h1 msg1_buffer) msg1_concat_s
+    /\ Seq.equal (as_seq h2 msg1_hash) msg1_hash_s
+    /\ Seq.equal (as_seq h3 input_hash) input_hash_s
+    /\ Seq.equal (as_seq h4 th2) th2_s
+  );
+
+  ST.pop_frame ();
+  ()
+// #pop-options
+
+let compute_th2_pre_hash #kcs ct_y k_auth_I msg1_hash th2
+  = ST.push_frame ();
+  (**) let h0 = ST.get () in
+
+  let msg1_hash_len = size (SpecCrypto.hash_size kcs) in
+  let input_len = kem_ciphertext_size_t kcs +! kem_shared_secret_size_t kcs +! msg1_hash_len in
+  let input_hash = create input_len (u8 0) in
+  concat_buff3 ct_y k_auth_I msg1_hash input_hash;
+  (**) let h1 = ST.get () in
+
+  do_hash kcs th2 input_len input_hash;
+  (**) let h2 = ST.get () in
+  (**) assert(
+    let input_hash_s = (as_seq h0 ct_y) @< (as_seq h0 k_auth_I) @< (as_seq h0 msg1_hash) in
+    Seq.equal (as_seq h1 input_hash) input_hash_s
+  );
+
+  ST.pop_frame ();
+  ()
+
+/// Transcript Hash 3
+let compute_th3 #kcs th2 ptx2 cred_r th3
+  = ST.push_frame ();
+  (**) let h0 = ST.get () in
+
+  let ptx2_buffer = create (plaintext2_size_t kcs) (u8 0) in
+  concat_ptx2 kcs ptx2 ptx2_buffer;
+  (**) let h1 = ST.get () in
+  
+  let input_len = (size (SpecCrypto.hash_size kcs)) +! (plaintext2_size_t kcs) +! (size SpecParser.cred_size) in
+  let input_hash = create input_len (u8 0) in
+  concat_buff3 th2 ptx2_buffer cred_r input_hash;
+  (**) let h2 = ST.get () in
+
+  do_hash kcs th3 input_len input_hash;
+  (**) let h3 = ST.get () in
+  (**) assert(
+    let input_hash_s = (as_seq h0 th2) @< (SpecParser.concat_ptx2 (plaintext2_eval h0 ptx2)) @< (as_seq h0 cred_r) in
+
+    Seq.equal (as_seq h2 input_hash) input_hash_s
+  );
+
+  ST.pop_frame ();
+  ()
+
+/// Transcript Hash 4
+let compute_th4 #kcs th3 ptx3 cred_i th4
+  = ST.push_frame ();
+  (**) let h0 = ST.get () in
+
+  let ptx3_buffer = create (plaintext3_size_t kcs) (u8 0) in
+  concat_ptx3 kcs ptx3 ptx3_buffer;
+  (**) let h1 = ST.get () in
+
+  let input_len = (size (SpecCrypto.hash_size kcs)) +! (plaintext3_size_t kcs) +! (size SpecParser.cred_size) in
+  let input_hash = create input_len (u8 0) in
+  concat_buff3 th3 ptx3_buffer cred_i input_hash;
+  (**) let h2 = ST.get () in
+
+  do_hash kcs th4 input_len input_hash;
+  (**) let h3 = ST.get () in
+  (**) assert(
+    let input_hash_s = (as_seq h0 th3) @< (SpecParser.concat_ptx3 (plaintext3_eval h0 ptx3)) @< (as_seq h0 cred_i) in
+
+    Seq.equal (as_seq h2 input_hash) input_hash_s
+  );
+  ST.pop_frame ();
+  ()
