src/kemedhoc/Impl.KEMEDHOC.TranscriptHash.fsti
@@ -1,0 +1,124 @@
+module Impl.KEMEDHOC.TranscriptHash
+
+(*HACL related modules*)
+// open Lib.RawIntTypes
+open Lib.IntTypes
+// open Lib.Sequence
+open Lib.ByteBuffer
+// lbuffer type, an immutable buffer with
+// length tag, is from this module
+// let lbuffer (a:Type0) (len:size_t) = lbuffer_t MUT a len
+// `live` and `disjoint` are also from this module.
+// Basically, HACL `Lib.Buffer` is a wrapper of `LowStar.Buffer`
+// and related LowStar memory models.
+open Lib.Buffer
+
+open Impl.EDHOC.Utilities
+
+(*LowStar related modules*)
+module B = LowStar.Buffer
+module ST = FStar.HyperStack.ST
+module HS = FStar.HyperStack
+module S = FStar.Seq
+module Seq = Lib.Sequence
+
+(*Specification modules*)
+module Spec = Spec.KEMEDHOC.TranscriptHash
+
+open Impl.KEMEDHOC.CryptoPrimitives
+open Impl.KEMEDHOC.Types
+open Impl.KEMEDHOC.Parser
+
+
+/// Transcript Hash 1
+val compute_th1:
+  #kcs: supportedKemCipherSuite
+  -> pk_X: kem_pub_key_buff kcs
+  -> ct_auth_R: kem_ciphertext_buff kcs
+  -> th1: hash_out_buff kcs
+  -> ST.Stack unit
+  (requires fun h0 ->
+    live h0 pk_X /\ live h0 ct_auth_R /\ live h0 th1
+    /\ B.all_disjoint [loc pk_X; loc ct_auth_R; loc th1]
+  )
+  (ensures fun h0 _ h1 ->
+    let th1_s = Spec.compute_th1 #kcs (as_seq h0 pk_X) (as_seq h0 ct_auth_R) in
+
+    modifies1 th1 h0 h1
+    /\ Seq.equal (as_seq h1 th1) th1_s
+  )
+
+/// Transcript Hash 2
+val compute_th2:
+  #kcs: supportedKemCipherSuite
+  -> ct_y: kem_ciphertext_buff kcs
+  -> k_auth_I: kem_shared_secret_buff kcs
+  -> msg1: message1 kcs
+  -> th2: hash_out_buff kcs
+  -> ST.Stack unit
+  (requires fun h0 ->
+    is_valid_message1 h0 msg1 /\ live h0 ct_y /\ live h0 k_auth_I /\ live h0 th2
+    /\ B.all_disjoint [loc ct_y; loc k_auth_I; loc th2; message1_union msg1]
+  )
+  (ensures fun h0 _ h1 ->
+    let th2_s = Spec.compute_th2 #kcs (as_seq h0 ct_y) (as_seq h0 k_auth_I) (message1_eval h0 msg1) in
+
+    modifies1 th2 h0 h1
+    /\ Seq.equal (as_seq h1 th2) th2_s
+  )
+
+val compute_th2_pre_hash:
+  #kcs: supportedKemCipherSuite
+  -> ct_y: kem_ciphertext_buff kcs
+  -> k_auth_I: kem_shared_secret_buff kcs
+  -> msg1_hash: hash_out_buff kcs
+  -> th2: hash_out_buff kcs
+  -> ST.Stack unit
+  (requires fun h0 ->
+    live h0 ct_y /\ live h0 k_auth_I /\ live h0 msg1_hash /\ live h0 th2
+    /\ B.all_disjoint [loc ct_y; loc k_auth_I; loc msg1_hash; loc th2]
+  )
+  (ensures fun h0 _ h1 ->
+    let th2_s = Spec.compute_th2_pre_hash #kcs (as_seq h0 ct_y) (as_seq h0 k_auth_I) (as_seq h0 msg1_hash) in
+
+    modifies1 th2 h0 h1
+    /\ Seq.equal (as_seq h1 th2) th2_s
+  )
+
+/// Transcript Hash 3
+val compute_th3:
+  #kcs: supportedKemCipherSuite
+  -> th2: hash_out_buff kcs
+  -> ptx2: plaintext2 kcs
+  -> cred_r: cred_buffer
+  -> th3: hash_out_buff kcs
+  -> ST.Stack unit
+  (requires fun h0 ->
+    is_valid_plaintext2 h0 ptx2 /\ live h0 th2 /\ live h0 cred_r /\ live h0 th3
+    /\ B.all_disjoint [loc th2; loc cred_r; loc th3; plaintext2_union ptx2]
+  )
+  (ensures fun h0 _ h1 ->
+    let th3_s = Spec.compute_th3 #kcs (as_seq h0 th2) (plaintext2_eval h0 ptx2) (as_seq h0 cred_r) in
+
+    modifies1 th3 h0 h1
+    /\ Seq.equal (as_seq h1 th3) th3_s
+  )
+
+/// Transcript Hash 4
+val compute_th4:
+  #kcs: supportedKemCipherSuite
+  -> th3 : hash_out_buff kcs
+  -> ptx3 : plaintext3 kcs
+  -> cred_i : cred_buffer
+  -> th4 : hash_out_buff kcs
+  -> ST.Stack unit
+  (requires fun h0 ->
+    is_valid_plaintext3 h0 ptx3 /\ live h0 th3 /\ live h0 cred_i /\ live h0 th4
+    /\ B.all_disjoint [loc th3; loc cred_i; loc th4; plaintext3_union ptx3]
+  )
+  (ensures fun h0 _ h1 ->
+    let th4_s = Spec.compute_th4 #kcs (as_seq h0 th3) (plaintext3_eval h0 ptx3) (as_seq h0 cred_i) in
+
+    modifies1 th4 h0 h1
+    /\ Seq.equal (as_seq h1 th4) th4_s
+  )
